a start on the stack_remove proof

compiler/backend/stack_removeScript.sml
@@ -8,63 +8,94 @@ val _ = new_theory "stack_remove";
 val word_offset_def = Define `
   word_offset n = n2w (dimindex (:'a) DIV 8 * n):'a word`;
 
+val store_list_def = Define `
+  store_list = [NextFree; EndOfHeap; HeapLength; OtherHeap;
+                AllocSize; Handler; Globals; ProgStart]`
+
 val store_pos_def = Define `
-  (store_pos name):num =
-    case name of
-    | HeapLength => 0
-    | NextFree => 1
-    | EndOfHeap => 2
-    | CurrHeap => 3
-    | OtherHeap => 4
-    | AllocSize => 5
-    | Handler => 6
-    | Globals => 7
-    | ProgStart => 8`
+  store_pos name =
+    case INDEX_FIND 0 (\n. n = name) store_list of
+    | NONE => 0n
+    | SOME (i,_) => i+1`
 
 val store_length_def = Define `
-  store_length = 8n`; (* must be even and <= store_pos n, for any n *)
+  store_length =
+    if EVEN (LENGTH store_list) then LENGTH store_list
+    else LENGTH store_list + 1`
 
 val store_offset_def = Define `
   store_offset name = 0w - word_offset (store_pos name)`;
 
 val stack_err_lab_def = Define `
-  stack_err_lab = 5:num`;
+  stack_err_lab = 5n`;
+
+val stack_err_stub_def = Define `
+  stack_err_stub = [Inst (Const 1 2w); Halt 1]`
+
+(*
+    k is stack pointer register
+    k+1 is base of store array (and last stack address)
+    k+2 is CurrHeap (which is kept in a register for improved speed)
+*)
+
+val move_def = Define `
+  move dest src = Inst (Arith (Binop Or dest src (Reg src)))`
+
+val max_stack_alloc_def = Define `
+  max_stack_alloc = 256n`;
+
+val single_stack_alloc_def = Define `
+  single_stack_alloc k n =
+    Seq (Inst (Arith (Binop Sub k k (Imm (word_offset n)))))
+        (JumpLess k (k+1) stack_err_lab)`
+
+val stack_alloc_def = tDefine "stack_alloc" `
+  stack_alloc k n =
+    if n = 0 then Skip else
+    if n <= max_stack_alloc then single_stack_alloc k n else
+      Seq (single_stack_alloc k max_stack_alloc)
+          (stack_alloc k (n - max_stack_alloc))`
+ (WF_REL_TAC `measure SND`
+  \\ fs [max_stack_alloc_def] \\ decide_tac)
 
 val comp_def = Define `
-  comp sp bp p =
+  comp k p =
     case p of
     (* remove store accesses *)
-    | Get r name => Inst (Mem Load r (Addr bp (store_offset name)))
-    | Set name r => Inst (Mem Store r (Addr bp (store_offset name)))
+    | Get r name =>
+        if name = CurrHeap then move r (k+2)
+        else Inst (Mem Load r (Addr (k+1) (store_offset name)))
+    | Set name r =>
+        if name = CurrHeap then move (k+2) r
+        else Inst (Mem Store r (Addr (k+1) (store_offset name)))
     (* remove stack operations *)
-    | StackFree n => Inst (Arith (Binop Add sp sp (Imm (word_offset n))))
-    | StackAlloc n => Seq (Inst (Arith (Binop Sub sp sp (Imm (word_offset n)))))
-                          (JumpLess sp bp stack_err_lab)
-    | StackStore r n => Inst (Mem Store r (Addr sp (word_offset n)))
-    | StackLoad r n => Inst (Mem Load r (Addr sp (word_offset n)))
-    | StackLoadAny r i => Seq (Inst (Arith (Binop Add r i (Reg sp))))
+    | StackFree n => Inst (Arith (Binop Add k k (Imm (word_offset n))))
+    | StackAlloc n => stack_alloc k n
+    | StackStore r n => Inst (Mem Store r (Addr k (word_offset n)))
+    | StackLoad r n => Inst (Mem Load r (Addr k (word_offset n)))
+    | StackLoadAny r i => Seq (Inst (Arith (Binop Add r i (Reg k))))
                               (Inst (Mem Load r (Addr r 0w)))
-    | StackStoreAny r i => Seq (Inst (Arith (Binop Add sp sp (Reg i))))
-                          (Seq (Inst (Mem Store r (Addr sp 0w)))
-                               (Inst (Arith (Binop Sub sp sp (Reg i)))))
-    | StackGetSize r => Inst (Arith (Binop Sub r sp (Reg bp)))
-    | StackSetSize r => Inst (Arith (Binop Add sp bp (Reg r)))
+    | StackStoreAny r i => Seq (Inst (Arith (Binop Add k k (Reg i))))
+                          (Seq (Inst (Mem Store r (Addr k 0w)))
+                               (Inst (Arith (Binop Sub k k (Reg i)))))
+    | StackGetSize r => Inst (Arith (Binop Sub r k (Reg (k+1))))
+    | StackSetSize r => Inst (Arith (Binop Add k (k+1) (Reg r)))
     (* for the rest, just leave it unchanged *)
-    | Seq p1 p2 => Seq (comp sp bp p1) (comp sp bp p2)
-    | If c r ri p1 p2 => If c r ri (comp sp bp p1) (comp sp bp p2)
+    | Seq p1 p2 => Seq (comp k p1) (comp k p2)
+    | If c r ri p1 p2 => If c r ri (comp k p1) (comp k p2)
     | Call ret dest exc =>
         Call (case ret of
               | NONE => NONE
-              | SOME (p1,lr,l1,l2) => SOME (comp sp bp p1,lr,l1,l2))
+              | SOME (p1,lr,l1,l2) => SOME (comp k p1,lr,l1,l2))
           dest (case exc of
                 | NONE => NONE
-                | SOME (p2,l1,l2) => SOME (comp sp bp p2,l1,l2))
+                | SOME (p2,l1,l2) => SOME (comp k p2,l1,l2))
     | p => p`
 
 val prog_comp_def = Define `
-  prog_comp sp bp (n,p) = (n,comp sp bp p)`
+  prog_comp k (n,p) = (n,comp k p)`
 
 val compile_def = Define `
-  compile (sp,bp) prog = MAP (prog_comp sp bp) prog`;
+  compile k prog = MAP (prog_comp k) prog`;
 
 val _ = export_theory();
