compiler/backend/bvp_to_wordScript.sml
@@ -8,9 +8,6 @@ val _ = Datatype `
             ; pad_bits : num (* in each pointer *)
             ; len_size : num (* size of length field in block header *) |>`
 
-val bytes_in_word_def = Define `
-  bytes_in_word = n2w (dimindex (:'a) DIV 8):'a word`;
-
 val adjust_var_def = Define `
   adjust_var n = 2 * n + 2:num`;
 
